ref_impl/src/verifier/fstar_files/NSMain__main_main.fst
@@ -8,25 +8,11 @@ open Util
 let bTypedStringType_BAnyType = (BTypedStringType BAnyType)
 let bRecordType_3BBoolType_BIntType_bTypedStringType_BAnyTypefalse = BRecordType false 3 (SCons "f" 2 (SCons "g" 1 (SCons "h" 0 SNil))) (SCons BBoolType 2 (SCons BIntType 1 (SCons bTypedStringType_BAnyType 0 SNil)))
 let bRecordType_2BBoolType_BIntTypefalse = BRecordType false 2 (SCons "f" 1 (SCons "g" 0 SNil)) (SCons BBoolType 1 (SCons BIntType 0 SNil))
+let bRecordType_2BIntType_BBoolTypefalse = BRecordType false 2 (SCons "f" 1 (SCons "k" 0 SNil)) (SCons BIntType 1 (SCons BBoolType 0 SNil))
 
 (* Constant Declarations *)
 
 (* Function Declarations *)
-val nSMain__selectF : (x:bosqueTerm{subtypeOf BBoolType (getType x)}) -> Tot (x:bosqueTerm{subtypeOf BIntType (getType x)})
-let nSMain__selectF x = 
-  if x then 
-    let _LoadConst = (BInt 0) in
-    let __tmp_0_2 = __tmp_0_1 in
-    let __ir_ret__ = __tmp_0_2 in
-    let _return_ = __ir_ret__ in
-    _return_
-  else 
-    let _LoadConst = (BInt 0) in
-    let __tmp_0_2 = __tmp_0 in
-    let __ir_ret__ = __tmp_0_2 in
-    let _return_ = __ir_ret__ in
-    _return_
-
 val nSMain__main : (x:bosqueTerm{subtypeOf BIntType (getType x)})
 let nSMain__main  = 
   let __tmp_0 = (BRecord 3 (SCons "f" 2 (SCons "g" 1 (SCons "h" 0 SNil))) (SCons (BBool true) 2 (SCons (BInt 2) 1 (SCons (BTypedString "hello" BAnyType) 0 SNil)))) in
@@ -46,16 +32,16 @@ let nSMain__main  =
   let _ = assert_norm(subtypeOf BIntType (getType __tmp_10_arg_0)) in
   let __tmp_10 = (BnSMain__Baz2 __tmp_10_arg_0 __tmp_10_arg_1 __tmp_10_arg_2) in
   let e = __tmp_10 in
-  let _MIRAccessFromField = (BInt 0) in
+  let _ = assert_norm(subtypeOf BnSMain__Baz2Type (getType e)) in
+  let __tmp_16 = (projectBnSMain__Baz2_f e) in
   let e2 = __tmp_16 in
-  let _MIRProjectFromTypeConcept = (BInt 0) in
+  let __fresh_name1NSMain__main = (projectBnSMain__Baz2_k e) in
+  let __fresh_name0NSMain__main = (projectBnSMain__Baz2_f e) in
+  let __tmp_19 = (BRecord 2 (SCons "f" 1 (SCons "k" 0 SNil)) (SCons __fresh_name0NSMain__main 1 (SCons __fresh_name1NSMain__main 0 SNil))) in
   let e3 = __tmp_19 in
-  let _MIRModifyWithFields = (BInt 0) in
+  let _MIRProjectFromTypeConcept = (BInt 0) in
   let e4 = __tmp_22 in
-  let _ = assert_norm(subtypeOf BBoolType (getType (BBool true))) in
-  let __tmp_24 = (nSMain__selectF (BBool true)) in
-  let f = __tmp_24 in
-  let __ir_ret__ = x_ProjectedRecord in
+  let __ir_ret__ = e2 in
   let _return_ = __ir_ret__ in
   _return_
 
